adapted proof for secure channel

theories/prob_eff_lang/probblaze/examples/DH_KE/new_schan_ri.v
@@ -1,4 +1,4 @@
-From iris.proofmode Require Import base proofmode classes.                        
+From iris.proofmode Require Import base proofmode classes.                          
 From iris.base_logic.lib Require Import  na_invariants.   
 From iris.algebra Require Import agree excl auth frac excl_auth.
 From iris.algebra.lib Require Import dfrac_agree.
@@ -11,7 +11,7 @@ From clutch.prob_eff_lang.probblaze Require Import def_dhke.
 From clutch.prob_eff_lang.probblaze Require Import dhke_channel.
 (*From clutch.prob_eff_lang.probblaze Require Import def_schannel.*)
 From clutch.prob_eff_lang.probblaze Require Import sem_types sem_row sem_sig sem_judgement sem_def.
-From clutch.prob_eff_lang.probblaze Require Import p_composition.
+From clutch.prob_eff_lang.probblaze Require Import p_composition. 
 From clutch.prob_eff_lang.probblaze Require Import newdef_schan.
 
 Import fingroup.
@@ -52,20 +52,20 @@ Section schan_security.
 
   (* Theories for the authenticated channel leaks *)
   (*-------------------------------------------------------------*)
-   (* Send TO Bob*)
+   (* Sent BY Bob TO Alice*)
    Program Definition LASendBob (leakauth1 leakauth2 : label) : iThy Σ :=
-  λ e1 e2, (λne Q,
-              ∃ m1 m2 : val,
-                ⌜e1 = (do: leakauth1 (SendV (m1, bob)))⌝%E ∗ 
-                           ⌜ e2 = do: leakauth2 (SendV (m2, bob)) ⌝%E ∗
-                                      □ Q (Val #()%V) (Val #()%V))%I.
-  Next Obligation. solve_proper. Qed.
-  (* Send TO Alice*)
-  Program Definition LASendAlice (leakauth1 leakauth2 : label) : iThy Σ :=
   λ e1 e2, (λne Q,
               ∃ m1 m2 : val,
                 ⌜e1 = (do: leakauth1 (SendV (m1, alice)))⌝%E ∗ 
                            ⌜ e2 = do: leakauth2 (SendV (m2, alice)) ⌝%E ∗
+                                      □ Q (Val #()%V) (Val #()%V))%I.
+  Next Obligation. solve_proper. Qed.
+  (* Sent BY Alice TO Bob*)
+  Program Definition LASendAlice (leakauth1 leakauth2 : label) : iThy Σ :=
+  λ e1 e2, (λne Q,
+              ∃ m1 m2 : val,
+                ⌜e1 = (do: leakauth1 (SendV (m1, bob)))⌝%E ∗ 
+                           ⌜ e2 = do: leakauth2 (SendV (m2, bob)) ⌝%E ∗
                                       □ Q (Val #()%V) (Val #()%V))%I.
   Next Obligation. solve_proper. Qed.
   (*Recv FROM bob*) 
@@ -225,12 +225,13 @@ Section schan_security.
   (*----------------------------------------------------------------------------*)
 
    Definition sem_ty_group : sem_ty Σ := (λ v1 v2, ∃ g : vgG, ⌜ v1 = g ⌝ ∗ ⌜ v2 = g ⌝)%I.
-  Notation "'𝔾'" := sem_ty_group. 
-  (*Program Definition bot_mono := {| pmono_prot_car := iThyBot ; pmono_prot_prop := _ |}.
-  Next Obligation. solve_proper. Defined.
+   Notation "'𝔾'" := sem_ty_group.
+  
+ (* Program Definition bot_mono := {| pmono_prot_car := iThyBot ; pmono_prot_prop := _ |}.
+  Next Obligation. iIntros (?). Defined.
  
-  Definition thy_sec_chan (l1 l2 : label) := @SemSig Σ bot_mono (l1,l2).
-  Program Definition thy_sec_row (channel leaksec getKey1 getKey2 schannel1 schannel2 : label) :=
+  Definition empty_thy (l1 l2 : label) := @SemSig Σ bot_mono (l1,l2).
+  Program Definition empty_thy_row (channel leaksec getKey1 getKey2 schannel1 schannel2 : label) :=
     SemRow [([channel; getKey1; schannel1] , [leaksec; getKey2; schannel2] , bot_mono)] _.*)
   Program Definition keyleak_mono (keyleak1 keyleak2 : label) := {| pmono_prot_car := iThySum (iThySum (KLeakSendAlice keyleak1 keyleak2) (KLeakRecvAlice keyleak1 keyleak2)) (iThySum (KLeakSendBob keyleak1 keyleak2) (KLeakRecvBob keyleak1 keyleak2)) ; pmono_prot_prop := _|}.
   Next Obligation.
@@ -241,9 +242,9 @@ Section schan_security.
    all: iDestruct "HR" as (??) "(#H1 & #H2)"; simpl; iSplit; first done; iSplit; first done; iModIntro; iSplitL " "; iApply "HΦ"; try (iApply "H1"); try (iApply "H2").
   Qed.
   Definition keyleak (keyleak1 keyleak2 : label) := @SemSig Σ (keyleak_mono keyleak1 keyleak2) (keyleak1, keyleak2).
-  Lemma keyleak_pers_mono_row (channel leaksec getKey1 schannel1 schannel2 keyleak1 keyleak2 : label) : ⊢ pers_mono_row (iLblSig_to_iLblThy [([channel; getKey1; schannel1; keyleak1] , [leaksec; schannel2; keyleak2] , keyleak keyleak1 keyleak2)]).
+  Lemma keyleak_pers_mono_row (keyleak1 keyleak2 : label) : ⊢ pers_mono_row (iLblSig_to_iLblThy [([keyleak1] , [keyleak2] , keyleak keyleak1 keyleak2)]).
   Proof. Admitted.
-  Definition keyleak_row (channel leaksec getKey1 schannel1 schannel2 keyleak1 keyleak2 : label) := SemRow [([channel; getKey1; schannel1; keyleak1] , [leaksec; schannel2; keyleak2] , keyleak keyleak1 keyleak2)] (keyleak_pers_mono_row channel leaksec getKey1 schannel1 schannel2 keyleak1 keyleak2).
+  Definition keyleak_row (keyleak1 keyleak2 : label) := SemRow [([keyleak1] , [keyleak2] , keyleak keyleak1 keyleak2)] (keyleak_pers_mono_row keyleak1 keyleak2).
  
   Program Definition leakauth_mono (leakauth1 leakauth2 : label) := {| pmono_prot_car := iThySum (iThySum (LASendAlice leakauth1 leakauth2) (LASendBob leakauth1 leakauth2)) (iThySum (LARecvAlice leakauth1 leakauth2) (LARecvBob leakauth1 leakauth2)) ; pmono_prot_prop := _ |}.
   Next Obligation.
@@ -259,8 +260,8 @@ Section schan_security.
   Lemma leakauth_pers_mono_row (leakauth1 leakauth2 : label) : ⊢ pers_mono_row (iLblSig_to_iLblThy [([leakauth1], [leakauth2], leakauth leakauth1 leakauth2)]).
   Proof. Admitted.
   Definition leakauth_row (leakauth1 leakauth2 : label) := SemRow [([leakauth1],[leakauth2] , leakauth leakauth1 leakauth2 )] (leakauth_pers_mono_row leakauth1 leakauth2).
-  Program Definition envsec_row (channel leaksec getKey1 schannel1 schannel2 keyleak1 keyleak2 leakauth1 leakauth2 : label) :=
-    sem_row_union (keyleak_row channel leaksec getKey1 schannel1 schannel2 keyleak1 keyleak2) (leakauth_row leakauth1 leakauth2).
+  Program Definition envsec_row (keyleak1 keyleak2 leakauth1 leakauth2 : label) :=
+    sem_row_union (keyleak_row keyleak1 keyleak2) (leakauth_row leakauth1 leakauth2).
 
   Program Definition sec_channel_mono (schannel1 schannel2 : label) := {| pmono_prot_car := iThySum (SendSecAlice schannel1 schannel2) (RecvSecBob schannel1 schannel2) ; pmono_prot_prop := _ |}.
   Next Obligation.
@@ -268,11 +269,16 @@ Section schan_security.
 
   Definition sec_channel (schannel1 schannel2 : label) := @SemSig Σ (sec_channel_mono schannel1 schannel2) (schannel1, schannel2).
 
-  Lemma sec_channel_pers_mono_row (getKey1 schannel1 schannel2 : label) : ⊢ pers_mono_row (iLblSig_to_iLblThy [([getKey1; schannel1] , [schannel2] , sec_channel schannel1 schannel2)]).
+  Lemma client_pers_mono_row (getKey1 schannel1 schannel2 : label) : ⊢ pers_mono_row (iLblSig_to_iLblThy [([getKey1; schannel1] , [schannel2] , sec_channel schannel1 schannel2)]).
+  Proof.
+  Admitted.
+
+  Lemma sec_channel_pers_mono_row (schannel1 schannel2 : label) : ⊢ pers_mono_row (iLblSig_to_iLblThy [([schannel1] , [schannel2], sec_channel schannel1 schannel2)]).
   Proof.
   Admitted.
   
-  Program Definition client_row (getKey1 schannel1 schannel2 : label) := SemRow [([getKey1; schannel1], [schannel2], sec_channel schannel1 schannel2)] (sec_channel_pers_mono_row getKey1 schannel1 schannel2) .
+  Program Definition sec_channel_row (schannel1 schannel2 : label) := SemRow [([schannel1], [schannel2], sec_channel schannel1 schannel2)] (sec_channel_pers_mono_row schannel1 schannel2).
+  Program Definition client_row (getKey1 schannel1 schannel2 : label) := SemRow [([getKey1; schannel1], [schannel2], sec_channel schannel1 schannel2)] (client_pers_mono_row getKey1 schannel1 schannel2) .
    Definition REAL_CHAN : val :=
     λ: "f",
     (F_OAUTH ||ₗ F_KE_L) (CHAN "f").
@@ -283,20 +289,20 @@ Lemma F_KE_CHAN_SIM (f1 f2 : val) (L : sem_row Σ) :
     sem_val_typed f1 f2 ((∀ᵣ θₕ, (((sem_ty_sum 𝟙 𝟙) -{ θₕ }-> (Option  𝔾)) × ((sem_ty_sum 𝟙 𝟙) -{ θₕ }-> (Option  𝔾))) -{ sem_row_union  θₕ L }-> 𝟙))%T -∗ 
     BREL REAL_CHAN f1
       ≤ CHAN_SIM (F_CHAN f2) <|⊥|> {{λ v1 v2,
-                                       ∀ (channel leaksec getKey1 schannel1 schannel2 leakauth1 leakauth2 keyleak1 keyleak2 : label),
-                                       BREL v1 ((λ: "m", do: leakauth1 (Send "m")), (λ: "m", do: leakauth1 (Recv "m")))%V (λ: "m", do: keyleak1 "m")%V ≤ v2 ((λ: "m", do: leakauth2 (Send "m")), (λ: "m", do: leakauth2 (Recv "m")))%V (λ: "m", do: keyleak2 "m")%V <| (iLblSig_to_iLblThy (envsec_row channel leaksec getKey1 schannel1 schannel2 leakauth1 leakauth2 keyleak1 keyleak2 )) ++ (iLblSig_to_iLblThy L) |> {{ (λ w1 w2, 𝟙%T w1 w2)}}}}.
+                                       ∀ (leakauth1 leakauth2 keyleak1 keyleak2 : label),
+                                       BREL v1 ((λ: "m", do: leakauth1 (Send "m")), (λ: "m", do: leakauth1 (Recv "m")))%V (λ: "m", do: keyleak1 "m")%V ≤ v2 ((λ: "m", do: leakauth2 (Send "m")), (λ: "m", do: leakauth2 (Recv "m")))%V (λ: "m", do: keyleak2 "m")%V <| (iLblSig_to_iLblThy (envsec_row keyleak1 keyleak2 leakauth1 leakauth2 )) ++ (iLblSig_to_iLblThy L) |> {{ (λ w1 w2, 𝟙%T w1 w2)}}}}.
 Proof with (repeat foldkont) using G.
   iIntros "Hrelf1f2".
   repeat simpl.
   unfold REAL_CHAN. brel_pures.
   unfold left_composition. brel_pures.
   unfold CHAN.
-  repeat simpl. brel_pures'. 
+  repeat simpl. brel_pures'.
   
   (*unfold CHAN_SIM, F_OAUTH.*)
   unfold F_CHAN, CHAN_SIM, F_KE_L, F_OAUTH. 
    
-  repeat simpl. brel_pures. iModIntro. iIntros (?????????).
+  repeat simpl. brel_pures. iModIntro. iIntros (????).
   brel_pures.
   iApply brel_alloctape_r. iIntros (α) "Hα". brel_pures_r. 
   iApply brel_alloc_r. iIntros (l_sim) "Hl_sim". brel_pures_r.
@@ -312,7 +318,7 @@ Proof with (repeat foldkont) using G.
   iApply brel_effect_r. iIntros (schannel_r) "Hschannel_r !>". brel_pures_r.
   brel_pures'. repeat simpl. brel_pures'.
   iApply brel_alloc_l. iIntros (l_rchan) "!>Hlrchan". brel_pures_l.
-  iApply brel_effect_l. iIntros (schannel_l) "!> Hschannel_l !>". brel_pures_l.
+  iApply brel_effect_l. iIntros (schannel_l) "!> Hschannel_l !>". brel_pures_l. 
   set (kl1 := ( match: "payload" with
            InjL "payload" =>
            let: "dst" := "payload" in
@@ -326,7 +332,7 @@ Proof with (repeat foldkont) using G.
                  InjL <> => "k" #()%V
                | InjR "x" =>
                  let: "enc_m" := xor "x" "m" in
-                 (λ: "m", do: channel' InjL "m")%V (InjL ("enc_m", bob));; "k" #()%V
+                 (λ: "m", do: channel' InjL "m")%V ("enc_m", bob);; "k" #()%V
                end
            | InjR "m" => "k" #()%V
            end
@@ -335,7 +341,7 @@ Proof with (repeat foldkont) using G.
          match: "key" with
            InjL <> => "k" (InjLV #()%V)
          | InjR "key" =>
-           let: "r" := (λ: "m", do: channel' InjR "m")%V (InjR "from") in
+           let: "r" := (λ: "m", do: channel' InjR "m")%V "from" in
            match: "r" with
              InjL <> => "k" (InjLV #()%V)
            | InjR "x" => let: "enc_m" := xor "key" "x" in "k" (InjR "enc_m")
@@ -373,16 +379,16 @@ Proof with (repeat foldkont) using G.
            let: "m" := Fst "dst" in
            let: "dst" := Snd "dst" in
            match: ! #l_fchan with
-             InjL <> => #l_fchan <- InjR "m";; (λ: "m", do: leaksec' InjL "m")%V (InjL "dst");; "k" #()%V
+             InjL <> => #l_fchan <- InjR "m";; (λ: "m", do: leaksec' InjL "m")%V "dst";; "k" #()%V
            | InjR "x" => "k" #()%V
            end
        | InjR "from" =>
-         let: "r" := (λ: "m", do: leaksec' InjR "m")%V (InjR "from") in
+         let: "r" := (λ: "m", do: leaksec' InjR "m")%V "from" in
          match: "r" with InjL <> => "k" (InjLV #()%V) | InjR "x" => "k" (InjR "x") end
                  end)%E).
   set (kr2 := (  match: "payload" with
          InjL "payload" =>
-           (λ: "m", do: keyleak2 "m")%V (InjL "payload");; 
+           (λ: "m", do: keyleak2 "m")%V (InjL bob);; 
            let: "r" := (λ: "m", do: keyleak2 "m")%V (InjR bob) in
            match: "r" with
              InjL <> => "k" (InjLV #()%V)
@@ -391,7 +397,7 @@ Proof with (repeat foldkont) using G.
                InjL <> =>
                  let: "m'" := #()%V;; rand(#lbl:α) #(S n'') in
                  let: "mA" := vexp g "m'" in
-                 #l_sim <- InjR "m'";; (λ: "m", do: leakauth2 Send "m")%V (InjL ("mA", bob));; "k" #()%V
+                 #l_sim <- InjR "m'";; (λ: "m", do: leakauth2 Send "m")%V ("mA", bob);; "k" #()%V
              | InjR "m" => "k" #()%V
              end
            end
@@ -401,7 +407,7 @@ Proof with (repeat foldkont) using G.
          match: "r" with
            InjL <> => "k" (InjLV #()%V)
          | InjR "x" =>
-           let: "rla" := (λ: "m", do: leakauth2 Recv "m")%V (InjR "from") in
+           let: "rla" := (λ: "m", do: leakauth2 Recv "m")%V "from" in
            match: "rla" with InjL <> => "k" (InjLV #()%V) | InjR "x" => "k" ! #l_sim end
          end
                  end )%E).
@@ -442,9 +448,44 @@ Proof with (repeat foldkont) using G.
               betaN).
    iSplitL  "Hlrchan Hlfchan"; [iNext; iFrame; iLeft; iFrame|].
    iIntros "#Hinvβ" .
-   iApply ((brel_exhaustion (f1 ((λ: "m", do: schannel_l InjL "m"),(λ: "m", do: schannel_l InjR "m"))%V) (f2 ((λ: "m", do: schannel_r InjL "m"),(λ: "m", do: schannel_r InjR "m"))%V) _ _ _ _ _ _ _ _ _) with "[Hrelf1f2]"); try simpl; try auto; try (apply sublist_subseteq); try (apply singleton_sublist_l);
+   (*set (f'1 := ( handle: f1 (λ: "m", do: schannel_l InjL "m", λ: "m", do: schannel_l InjR "m")%V with
+     | effect schannel_l "payload", rec "k" as multi => kl1
+               | return "y" => #()%V end)%E).
+   set (f'2 := ( handle: f2 (λ: "m", do: schannel_r InjL "m", λ: "m", do: schannel_r InjR "m")%V with
+     | effect schannel_r "payload", rec "k" as multi => kr1
+     | return "y" => #()%V
+                 end)%E).
+   iApply brel_new_theory.
+   iApply (brel_add_label_l with "HgK").
+   iApply (brel_add_label_l with "Hchannel").
+   iApply (brel_add_label_r with "Hleaksec").
+   
+   iApply ((brel_exhaustion f'1 f'2 _ _ _ _ _ _ _ _ _ )); try simpl.
+   { admit.}
+   { admit.}
+   { 
+   About brel_exhaustion.
+   unfold f'1, f'2.*)
+   iApply brel_new_theory.
+   iApply (brel_add_label_l with "Hschannel_l").
+   iApply (brel_add_label_r with "Hschannel_r").
+   iApply (brel_add_label_l with "HgK").
+   iApply (brel_add_label_l with "Hchannel").
+   iApply (brel_add_label_r with "Hleaksec").
+   set (X :=  iLblSig_to_iLblThy [([schannel_l] , [schannel_r] , sec_channel schannel_l schannel_r)]).
+   set (R := (λ u1 u2 : val, 𝟙%T u1 u2)).
+   set (X' := sec_channel schannel_l schannel_r).
+   (*iAssert  (brel ⊤ (f1 (λ: "m", do: schannel_l InjL "m", λ: "m", do: schannel_l InjR "m")%V)
+    (f2 (λ: "m", do: schannel_r InjL "m", λ: "m", do: schannel_r InjR "m")%V)
+    (([channel'; getKey'; schannel_l], [leaksec'; schannel_r], X)
+     :: ([keyleak1], [keyleak2], keyleak keyleak1 keyleak2)
+        :: ([leakauth1], [leakauth2], leakauth leakauth1 leakauth2) :: iLblSig_to_iLblThy L)
+    R) as "Hrelf1f2mono".*)
+   About brel_exhaustion.
+   iApply ((brel_exhaustion (f1 ((λ: "m", do: schannel_l InjL "m"),(λ: "m", do: schannel_l InjR "m"))%V) (f2 ((λ: "m", do: schannel_r InjL "m"),(λ: "m", do: schannel_r InjR "m"))%V) _ _ X' _ _ R _ _ _) with "[Hrelf1f2]"); try simpl; try auto; try (apply sublist_subseteq); try (apply singleton_sublist_l);
      try (apply list_elem_of_In); try simpl; try auto; try (repeat (eapply sublist_skip)) ; try eapply sublist_nil_l.
-   iLöb as "IH".
+   { admit.}
+   iLöb as "IH". 
    iSplit; [iIntros (v1 v2) "%Hv1v2"; iModIntro; brel_pures; iModIntro; done |]. 
    iIntros (?????) "!# %Hk1 %Hk2 HXQ #Hrel".
    iDestruct "HXQ" as "[HSendAlice | HRecvBob]".
@@ -462,7 +503,7 @@ Proof with (repeat foldkont) using G.
          (* First message to be sent by the secure channel*)
         ++  iApply (brel_load_r _ _ _ _ [HandleCtx _ _ _ _ _ ; CaseCtx _ _] with "Hl_fchan").
              iIntros "Hl_fchan".
-             iApply (brel_load_l _ _ _  [HandleCtx Deep MS channel _ _ ; HandleCtx Deep MS getKey1 _ _; CaseCtx _ _] with "Hl_rchan").
+             iApply (brel_load_l _ _ _  [HandleCtx Deep MS channel' _ _ ; HandleCtx Deep MS getKey' _ _; CaseCtx _ _] with "Hl_rchan").
              iIntros "!>Hl_rchan". brel_pures.
              simpl. brel_pures. 
              iApply (brel_store_r _ _ _ _ [HandleCtx _ _ _ _ _ ; AppRCtx _] with "Hl_fchan"). iIntros "Hl_fchan".
@@ -477,40 +518,50 @@ Proof with (repeat foldkont) using G.
              iModIntro.
              iApply brel_na_close. iFrame.
              iSplitL; [iModIntro; iRight; iFrame "#"|].
-             set (keytheory := [([keyleak1], [keyleak2],
+            (* set (keytheory := [([keyleak1], [keyleak2],
          iThySum (iThySum KLeakSendAlice KLeakRecvAlice)
-           (iThySum KLeakSendBob KLeakRecvBob))]).
-            set (M := (([channel; getKey1; schannel1], [leaksec; schannel2; getKey2], iThyBot)
-        :: ([leakauth1], [leakauth2],
-             iThySum (iThySum LASendAlice LASendBob) (iThySum LARecvAlice LARecvBob)) :: L)).
+           (iThySum KLeakSendBob KLeakRecvBob))]).*)
+             (*set (keytheory := [([keyleak1], [keyleak2], keyleak keyleak1 keyleak2)]).*)
+            (*set (M := (([channel'; getKey'; schannel_l], [leaksec'; schannel_r], iThyBot)
+        :: ([leakauth1], [leakauth2], leakauth leakauth1 leakauth2) :: (iLblSig_to_iLblThy L))).
             set (N := (([channel; getKey1; schannel1], [leaksec; schannel2; getKey2], iThyBot)
      :: ([keyleak1], [keyleak2],
          iThySum (iThySum KLeakSendAlice KLeakRecvAlice)
            (iThySum KLeakSendBob KLeakRecvBob))
         :: ([leakauth1], [leakauth2],
-             iThySum (iThySum LASendAlice LASendBob) (iThySum LARecvAlice LARecvBob)) :: L)).
+             iThySum (iThySum LASendAlice LASendBob) (iThySum LARecvAlice LARecvBob)) :: L)).*)
             simpl.
             repeat foldkont.
             simpl.
-             set (kontleftbind := (let: "r" := do: keyleak1 InjR bob in
+            set (kontleftbind :=
+             (let: "r" := (λ: "m", do: keyleak1 "m")%V (InjR bob) in
              match: "r" with
                InjL <> => kont (InjLV #()%V)
              | InjR "w" => kont (InjR (vgval (g ^+ n)))
              end)%E).
-           set (kontrightbind := (let: "r" := do: keyleak2 InjR bob in
+            set (kontrightbind := (let: "r" := (λ: "m", do: keyleak2 "m")%V (InjR bob) in
      match: "r" with
        InjL <> => kont0 (InjLV #()%V)
      | InjR "x" =>
        match: ! #l_sim with
          InjL <> =>
            let: "m'" := #()%V;; rand(#lbl:α) #(S n'') in
-           let: "mA" := g ^ "m'" in
+           let: "mA" := vexp g "m'" in
            #l_sim <- InjR "m'";; 
-           (do: leakauth2 InjL ("mA", bob));; kont0 #()%V
+           (λ: "m", do: leakauth2 Send "m")%V (InjL ("mA", bob));; kont0 #()%V
        | InjR "m" => kont0 #()%V
        end
      end)%E).
-           iApply (brel_bind'' [HandleCtx Deep _ _ _ _; AppRCtx _] [AppRCtx _] keytheory M N  (λ v1 v2 : val, ⌜v1 = v2⌝%I) (Do keyleak1 (InjLV bob)) (Do keyleak2 (InjLV bob))).
+            About brel_bind''.
+            set (keytheory := iLblSig_to_iLblThy [([keyleak1], [keyleak2], keyleak keyleak1 keyleak2)]).
+            set (leaktheory := (iLblSig_to_iLblThy [([leakauth1], [leakauth2], leakauth leakauth1 leakauth2)])).
+            About leaktheory.
+            (*set (M := [([channel'; getKey'; schannel_l], [leaksec'; schannel_r], iThyBot Σ)]).*)
+            About brel_bind''.
+            set (M := [([channel'; getKey'; schannel_l], [leaksec'; schannel_r], @iThyBot Σ)] ++ leaktheory ++ (iLblSig_to_iLblThy L)).
+            set (N := [([channel'; getKey'; schannel_l], [leaksec'; schannel_r], @iThyBot Σ)] ++ keytheory ++ leaktheory ++ (iLblSig_to_iLblThy L)).
+           (* iApply (brel_bind'' [HandleCtx Deep _ _ _ _; AppRCtx _] [AppRCtx _] keytheory [([channel'; getKey'; schannel_l], [leaksec'; schannel_r], iThyBot)] (([leakauth1], [leakauth2], leakauth leakauth1 leakauth2) :: iLblSig_to_iLblThy L)  (λ v1 v2 : val, ⌜v1 = v2⌝%I) (Do keyleak1 (InjLV bob)) (Do keyleak2 (InjLV bob))).*)
+            iApply (brel_bind'' [HandleCtx Deep _ _ _ _; AppRCtx _] [AppRCtx _] keytheory M N (𝟙%T) (Do keyleak1 (InjLV bob)) (Do keyleak2 (InjLV bob))).
              { simpl. unfold M. repeat (rewrite -> labels_l_cons). set_solver. }
              { simpl. apply list_subseteq_nil. }
              { simpl. unfold M. unfold N. iApply to_iThy_le_intro'. eapply Permutation_submseteq.
@@ -521,15 +572,17 @@ Proof with (repeat foldkont) using G.
                 iExists _, _, [], [],_.
                 do 2 (iSplit; [done|]; iSplit; [iPureIntro; apply _|]).
                 iSplitL;  [|by iIntros "!>" (??) "H"; iApply "H"].
-                iRight. iLeft. simpl.
+                iRight. iLeft. simpl. 
                 repeat (iSplit; try (iPureIntro); try (unfold SendV); try reflexivity).
                 iModIntro.
                 iApply brel_value.
                 iIntros "$ !>". brel_pures.
-                About brel_learn.
-                iAssert (distinct' (LblClients ++ L)) as "%Hdistinct".
-                { unfold LblClients. admit. }
-                iApply (brel_bind'' _ _ keytheory M N  (λ v1 v2 : val, ⌜v1 = v2⌝%I) (Do keyleak1 (InjRV bob)) (Do keyleak2 (InjRV bob))).
+                (*About brel_learn.*)
+                About distinct'.
+                (*iAssert (distinct' (LblClients ++ L)) as "%Hdistinct".*)
+                iAssert (distinct' N) as "%Hdistinct".
+                { unfold N. admit. }
+                iApply (brel_bind'' _ _ keytheory M N 𝟙%T (Do keyleak1 (InjRV bob)) (Do keyleak2 (InjRV bob))).
                 { simpl. unfold M.  repeat (rewrite -> labels_l_cons). set_solver. }
                 { simpl. apply list_subseteq_nil. }
                 { simpl. unfold M. unfold N. iApply to_iThy_le_intro'. eapply Permutation_submseteq.
@@ -554,18 +607,20 @@ Proof with (repeat foldkont) using G.
                   +++ iApply brel_value.
                       iIntros "$ !>". brel_pures.
                       { simpl. unfold distinct in Hdistinct. destruct Hdistinct.
-                        unfold distinct_l in H1. unfold LblClients in H1. simpl in H1.
+                        unfold distinct_l in H1. (*unfold LblClients in H1. simpl in H1.*)
+                        unfold N in H1. simpl in H1.
                         repeat (rewrite -> labels_l_cons in H1).
                         eapply NoDup_app in H1.
                         eapply NoDup_cons_1_1. destruct H1 as [H1' H2'].
-                        apply (NoDup_app [channel; getKey1] [schannel1]) in H1'.
+                        apply (NoDup_app [channel'; getKey'] [schannel_l]) in H1'.
                         destruct H1' as [H1' H2'']. apply H1'.}
                       { simpl.
                         iApply (brel_na_inv _ _ alphaN); first set_solver.
                         iFrame "Hinvα".
                         iIntros "([ (>Hα & >Hl_sim & >Hl_auth) | (#>Hα & #>Hl_sim & #>Hl_auth) ] & Hclose)". 
-                        (*first message ot be sent by the authenticated channel*)
-                        - iApply (brel_load_l _ _ _ [CaseCtx _ _] with "Hl_auth"). 
+                        (*first message to be sent by the authenticated channel*)
+                        - 
+                          iApply (brel_load_l _ _ _ [CaseCtx _ _] with "Hl_auth"). 
                           (*iIntros "HvN HdN".
                           iApply (rel_load_l_mask [CaseCtx _ _]).*)                                          
                           iIntros "!> Hl_auth".
@@ -595,11 +650,11 @@ Proof with (repeat foldkont) using G.
                           iSplitL; [iModIntro; iRight; iFrame "#"|].
                           simpl.
                           brel_pures.
-                          set (leakatheory := [([leakauth1], [leakauth2],
+                         (* set (leakatheory := [([leakauth1], [leakauth2],
            iThySum (iThySum LASendAlice LASendBob)
-             (iThySum LARecvAlice LARecvBob))]).
-                          iApply (brel_bind _ _ _ leakatheory N _ (Do leakauth1 (InjLV (xor "x" "m", bob))) (Do leakauth2 (InjLV (vgval (g ^+ n) , bob)))).
-                          { simpl. unfold leakatheory. auto.
+             (iThySum LARecvAlice LARecvBob))]).*)
+                          iApply (brel_bind _ _ _ leaktheory N _ (Do leakauth1 (InjLV (xor "x" "m", bob))) (Do leakauth2 (InjLV (vgval (g ^+ n) , bob)))).
+                          { simpl. unfold leaktheory. auto.
                             unfold traversable. simpl.
                             About brel_bind.
                             Search traversable.
@@ -607,18 +662,18 @@ Proof with (repeat foldkont) using G.
                             iIntros (e1 e2 Q0).
                              admit. }
                           { simpl. auto. admit. }
-                          { iApply (brel_introduction' [leakauth1] [leakauth2]); try (unfold leakatheory);
+                          { iApply (brel_introduction' [leakauth1] [leakauth2]); try (unfold leaktheory);
                             try (apply list_elem_of_here).
                            iExists _, _, [], [],_.
                 do 2 (iSplit; [done|]; iSplit; [iPureIntro; apply _|]).
                 iSplitL;  [|by iIntros "!>" (??) "H"; iApply "H"].
                 iLeft. iLeft. simpl.
-                iExists _,_. repeat (iSplit; try (iPureIntro); try (unfold SendV); try reflexivity).
+                iExists _,_. repeat (iSplit; try (iPureIntro); try (unfold SendV); try reflexivity). 
                 iModIntro. iApply brel_value. iIntros "$ !>".
                 brel_pures.
                 iApply (brel_exhaustion (fill k1' #()%V) (fill k2' #()%V)).
                             { simpl. auto. }
-                            { simpl. auto. admit. }
+                            { simpl. auto. (*admit.*) }
                             { iApply "Hrel". iApply "HmQ". }
                             { iApply "IH". }          }                                                   
                       (*a message has already been sent by the authenticated channel*)
@@ -632,7 +687,7 @@ Proof with (repeat foldkont) using G.
                             brel_pures.
                             iApply (brel_exhaustion (fill k1' #()%V) (fill k2' #()%V)).
                             { simpl. auto. }
-                            { simpl. auto. admit. }
+                            { simpl. auto. (*admit.*) }
                             { iApply "Hrel". iApply "HmQ". }
                             { iApply "IH". } } } }
          (* A message has already been sent by the secure channel*)
@@ -646,7 +701,7 @@ Proof with (repeat foldkont) using G.
            brel_pures.
            iApply (brel_exhaustion (fill k1' #()%V) (fill k2' #()%V)).
            { simpl. auto. }
-           { simpl. auto. admit. }
+           { simpl. auto. (*admit.*) }
            { iApply "Hrel". iApply "HmQ". }
            { iApply "IH". }
      (* Recieved by Bob *)
@@ -654,7 +709,12 @@ Proof with (repeat foldkont) using G.
         rewrite -> He1. rewrite -> He2. brel_pures.
         { simpl. admit. }
         { simpl. admit. }
-        set (N := (([channel; getKey1; schannel1], [leaksec; schannel2; getKey2],
+         set (keytheory := iLblSig_to_iLblThy [([keyleak1], [keyleak2], keyleak keyleak1 keyleak2)]).
+         set (leaktheory := (iLblSig_to_iLblThy [([leakauth1], [leakauth2], leakauth leakauth1 leakauth2)])).
+         set (M := [([channel'; getKey'; schannel_l], [leaksec'; schannel_r], @iThyBot Σ)]).
+         (* ++ leaktheory ++ (iLblSig_to_iLblThy L)) *)
+         set (N := [([channel'; getKey'; schannel_l], [leaksec'; schannel_r], @iThyBot Σ)] ++ keytheory ++ leaktheory ++ (iLblSig_to_iLblThy L)).
+       (* set (N := (([channel; getKey1; schannel1], [leaksec; schannel2; getKey2],
       iThyBot)
      :: ([keyleak1], [keyleak2],
          iThySum (iThySum KLeakSendAlice KLeakRecvAlice)
@@ -667,13 +727,13 @@ Proof with (repeat foldkont) using G.
          iThySum (iThySum KLeakSendAlice KLeakRecvAlice)
            (iThySum KLeakSendBob KLeakRecvBob))]).
         set (M := [([channel; getKey1; schannel1],
-                 [leaksec; schannel2; getKey2], SecChannelThy)]).
-        iApply (brel_bind'' _ _ keyleakthy M N _ (Do keyleak1 (InjLV bob)) (Do keyleak2 (InjLV bob))).
+                 [leaksec; schannel2; getKey2], SecChannelThy)]).*)
+        iApply (brel_bind'' _ _ keytheory M N _ (Do keyleak1 (InjLV bob)) (Do keyleak2 (InjLV bob))).
         { simpl. unfold M. admit. }
         { simpl. admit. }
         { admit. }
         {  iApply (brel_introduction' [keyleak1] [keyleak2]).
-                1: { unfold keyleakthy.
+                1: { unfold keytheory.
                      eapply list_elem_of_here. }
                 iExists _, _, [], [],_.
                 do 2 (iSplit; [done|]; iSplit; [iPureIntro; apply _|]).
@@ -682,12 +742,12 @@ Proof with (repeat foldkont) using G.
                 repeat (iSplit; try (iPureIntro); try (unfold SendV); try reflexivity).
                 iModIntro. iApply brel_value. 
                 iIntros "$ !>". brel_pures.
-                iApply (brel_bind'' _ _ keyleakthy M N _ (Do keyleak1 (InjRV bob)) (Do keyleak2 (InjRV bob))).
+                iApply (brel_bind'' _ _ keytheory M N _ (Do keyleak1 (InjRV bob)) (Do keyleak2 (InjRV bob))).
                 { simpl. unfold M. admit. }
                 { simpl. admit. }
                 { admit. }
                 {  iApply (brel_introduction' [keyleak1] [keyleak2]).
-                1: { unfold keyleakthy.
+                1: { unfold keytheory.
                      eapply list_elem_of_here. }
                 iExists _, _, [], [],_.
                 do 2 (iSplit; [done|]; iSplit; [iPureIntro; apply _|]).
@@ -698,19 +758,19 @@ Proof with (repeat foldkont) using G.
                 (* Key not received by Bob*)
                    ++ iApply (brel_exhaustion (fill k1'(InjLV #()%V)) (fill k2' (InjLV #()%V))). 
                       { simpl. auto. }
-                      { simpl. admit. }
+                      { simpl. auto. (*admit.*) }
                       { iApply "Hrel". iApply "HmQ". }
                       { iApply "IH". }
                       (* Key received by Bob *)
                    ++  simpl. admit.
-                   ++ set (leakauththy := [([leakauth1], [leakauth2],
-                       iThySum (iThySum LASendAlice LASendBob) (iThySum LARecvAlice LARecvBob))]).
-                      iApply (brel_bind'' _ _ leakauththy _ N _ (Do leakauth1 (InjRV bob)) (Do leakauth2 (InjRV bob))).
+                   ++ (*set (leakauththy := [([leakauth1], [leakauth2],
+                       iThySum (iThySum LASendAlice LASendBob) (iThySum LARecvAlice LARecvBob))]).*) 
+                      iApply (brel_bind'' _ _ leaktheory M N _ (Do leakauth1 (InjRV bob)) (Do leakauth2 (InjRV bob))).
                       { simpl. admit. }
                       { simpl. admit. }
                       { admit. }
                       { iApply (brel_introduction' [leakauth1] [leakauth2]).
-                        1: { unfold leakauththy.
+                        1: { unfold leaktheory.
                              eapply list_elem_of_here. }
                         simpl.
                         iExists _, _, [], [],_.
@@ -763,7 +823,7 @@ Proof with (repeat foldkont) using G.
                           { simpl. auto. }
                           { simpl. admit. }
                           { iApply "Hrel". iApply "HmQ". }
-                          {iApply "IH". }*)
+                          {iApply "IH". }
 
 Admitted.
 
